src/Dafny/examples/fs/byte_fs.dfy
@@ -1,0 +1,24 @@
+include "fs.dfy"
+
+module ByteFs {
+  import opened Fs
+  import opened Machine
+
+  // TODO: implement this on top of the lower-level API in fs.dfy
+
+  function inode_data(sz: nat, blks: seq<Block>): (bs:seq<byte>)
+    requires forall i:nat | i < |blks| :: is_block(blks[i])
+    requires |blks| == Round.div_roundup_alt(sz, 4096)
+    ensures |bs| == sz
+  {
+    if sz % 4096 == 0 then (
+      C.concat_homogeneous_spec(blks, 4096);
+      C.concat(blks)
+      )
+    else (
+      C.concat_homogeneous_spec(C.without_last(blks), 4096);
+      C.concat(C.without_last(blks)) +
+      C.last(blks)[..sz % 4096]
+      )
+  }
+}
