src/Dafny/examples/fs/kinds.dfy
@@ -1,0 +1,109 @@
+include "../../jrnl/jrnl.s.dfy"
+
+module FsKinds {
+  import Arith
+  import opened Machine
+  import opened JrnlSpec
+  import opened Kinds
+
+  type Ino = uint64
+
+  predicate blkno_ok(blkno: Blkno) { blkno < 4096*8 }
+  predicate ino_ok(ino: Blkno) { ino < 32 }
+
+  // disk layout, in blocks:
+  //
+  // 513 for the jrnl
+  // 1 inode block (32 inodes)
+  // 1 bitmap block
+  // 4096*8 data blocks
+  const NumBlocks: nat := 513 + 1 + 1 + 4096*8
+    // if you want to make a disk for the fs 40,000 blocks is a usable number
+  lemma NumBlocks_upper_bound()
+    ensures NumBlocks < 40_000
+  {}
+
+  const InodeBlk: Blkno := 513
+  const DataAllocBlk: Blkno := 514
+
+  function method InodeAddr(ino: Ino): (a:Addr)
+    requires ino_ok(ino)
+    ensures a in addrsForKinds(fs_kinds)
+  {
+    kind_inode_size();
+    assert fs_kinds[InodeBlk] == KindInode;
+    Arith.mul_assoc(ino as nat, 128, 8);
+    Arith.mul_r_strictly_incr(ino as nat, 128*8, 32);
+    assert ino*128*8 < 4096*8;
+    Arith.mul_mod(ino as nat, 128*8);
+    assert kindSize(KindInode) == 128*8;
+    Addr(InodeBlk, ino*128*8)
+  }
+  function method DataBitAddr(bn: uint64): Addr
+    requires blkno_ok(bn)
+  {
+    Addr(DataAllocBlk, bn)
+  }
+  function method DataBlk(bn: uint64): (a:Addr)
+    requires blkno_ok(bn)
+    ensures a in addrsForKinds(fs_kinds)
+  {
+    assert fs_kinds[513+2+bn] == KindBlock;
+    assert kindSize(KindBlock) == 4096*8;
+    Arith.zero_mod(4096*8);
+    Addr(513+2+bn, 0)
+  }
+
+  const fs_kinds: map<Blkno, Kind> :=
+    // NOTE(tej): trigger annotation suppresses warning (there's nothing to
+    // trigger on here, but also nothing is necessary)
+    map blkno: Blkno {:trigger} |
+      513 <= blkno as nat < NumBlocks
+      :: (if blkno == InodeBlk
+      then KindInode
+      else if blkno == DataAllocBlk
+        then KindBit
+        else KindBlock) as Kind
+
+  lemma fs_kinds_valid()
+    ensures kindsValid(fs_kinds)
+  {}
+
+  lemma blkno_bit_inbounds(jrnl: Jrnl)
+    requires jrnl.Valid()
+    requires jrnl.kinds == fs_kinds
+    ensures forall bn :: blkno_ok(bn) ==> DataBitAddr(bn) in jrnl.data && jrnl.size(DataBitAddr(bn)) == 1
+  {
+    forall bn | blkno_ok(bn)
+      ensures DataBitAddr(bn) in jrnl.data
+    {
+      ghost var addr := DataBitAddr(bn);
+      jrnl.in_domain(addr);
+      jrnl.has_size(addr);
+    }
+  }
+
+  lemma inode_inbounds(jrnl: Jrnl, ino: Ino)
+    requires jrnl.Valid()
+    requires jrnl.kinds == fs_kinds
+    requires ino_ok(ino)
+    ensures InodeAddr(ino) in jrnl.data && jrnl.size(InodeAddr(ino)) == 8*128
+  {
+    kind_inode_size();
+    ghost var addr := InodeAddr(ino);
+    jrnl.in_domain(addr);
+    jrnl.has_size(addr);
+  }
+
+  lemma datablk_inbounds(jrnl: Jrnl, bn: Blkno)
+    requires jrnl.Valid()
+    requires jrnl.kinds == fs_kinds
+    requires blkno_ok(bn)
+    ensures DataBlk(bn) in jrnl.data && jrnl.size(DataBlk(bn)) == 8*4096
+  {
+    ghost var addr := DataBlk(bn);
+    jrnl.in_domain(addr);
+    jrnl.has_size(addr);
+  }
+
+}
